src/tls/TLS.Handshake.Server.fsti
@@ -4,33 +4,32 @@ open Mem
 open TLSConstants
 open TLSError
 open FStar.HyperStack.ST
-open TLS.Handshake.State
 
-module B = FStar.Bytes
 module CH = Parsers.ClientHello
 module E = Extensions
 module HSM = HandshakeMessages
 module HMAC = Old.HMAC.UFCMA
 module KS = Old.KeySchedule
-module HSL = HandshakeLog
 module Nego = Negotiation
 module HS = FStar.HyperStack
 module H = Hashing.Spec
 
+type hs = TLS.Handshake.Machine.server 
+
 val server_ClientHello2:
   hs: hs ->
-  ch1: HSM.clientHello ->
+  ch1: HSM.ch ->
   hrr: HSM.hrr ->
-  ch2: HSM.clientHello ->
-  app_cookie: B.bytes ->
-  ST incoming
+  ch2: HSM.ch ->
+  app_cookie: Bytes.bytes ->
+  ST TLS.Handshake.Receive.incoming
   (requires fun h -> True)
   (ensures fun h0 _ h1 -> True)
   
 val server_ClientHello:
   hs: hs ->
-  ch: HSM.clientHello ->
-  ST incoming
+  ch: HSM.ch ->
+  ST TLS.Handshake.Receive.incoming
   (requires (fun h -> True))
   (ensures (fun h0 i h1 -> True))
 
@@ -43,23 +42,23 @@ val server_ClientCCS1:
   hs: hs ->
   cke: cke_t ->
   digestCCS1: H.anyTag ->
-  St incoming
+  St TLS.Handshake.Receive.incoming
 
 // Received [CF] (full handshake)
 val server_ClientFinished:
   hs: hs ->
-  cvd: B.bytes ->
+  cvd: Bytes.bytes ->
   digestCCS: H.anyTag ->
   digestCF: H.anyTag ->
-  St incoming
+  St TLS.Handshake.Receive.incoming
 
 // Received [CF] (resumption)
 val server_ClientFinished2:
   hs: hs ->
-  cvd: B.bytes ->
+  cvd: Bytes.bytes ->
   digestSF: H.anyTag ->
   digestCF: H.anyTag ->
-  St incoming
+  St TLS.Handshake.Receive.incoming
 
 (*** TLS 1.3 ***)
 
@@ -70,16 +69,16 @@ val server_ServerFinished_13:
 val server_EOED:
   hs: hs ->
   digestEOED: H.anyTag ->
-  St incoming
+  St TLS.Handshake.Receive.incoming
 
 val server_Ticket13:
   hs: hs ->
-  app_data: B.bytes ->
+  app_data: Bytes.bytes ->
   St unit
 
 val server_ClientFinished_13: hs ->
-  cvd: B.bytes ->
+  cvd: Bytes.bytes ->
   digest_SF: H.anyTag ->
   digest_CF: H.anyTag ->
-  client_cert: option (HSM.certificate13 * HSM.certificateVerify13 * H.anyTag) ->
-  St incoming
+  client_cert: option (HSM.certificate13 & HSM.certificateVerify13 & H.anyTag) ->
+  St TLS.Handshake.Receive.incoming
